\chapter{AdaBoost}

\section{Loss Function}
Exponential Loss Function:
\begin{equation}
L(y,f(x))=\exp[-yf(x)]
\end{equation}

\section{Objective Function}

\begin{equation}
(\alpha_m,G_m(x))= \underset{\alpha,G}{\operatorname{argmin}} \sum_{i=1}^N \exp{[-y_i(f_{m-1}(x_i)+\alpha G(x_i))]}
\end{equation}

equals with:
\begin{equation}
(\alpha_m,G_m(x))= \underset{\alpha,G}{\operatorname{argmin}} \sum_{i=1}^N {\bar{w}}_{mi} \exp{(-y_i \alpha G(x_i))}
\end{equation}

\section{Algorithm}
\subsection{input}
$T=\{(x_1,y_1),(x2,y2),\dotsc,(x_N,y_N) \};\ x_i\in \mathbb{R};\ y_i \in \{-1,+1\};$\ Weak\ Learner.
\subsection{output}
Final Learner:\ G(x)

\subsection{Algorithm}
\begin{enumerate}
\item Initialize\ the\ weights'\ distribution\ of\ training\ data(when\ m=1):
\begin{equation}
D_1=(w_{11},w_{12},\dotsc,w_{1n}}),w_{in}=\frac{1}{N},\ i=1,2,\dotsc,N
\end{equation}
\item iterate $m=1,2,\dotsc,M$


\subitem a. Train\ the\ weak\ learner\ with\ the\ weights'\ distribution\ $D_m$\ and\ get\ the\ classifier\ $G_m(x)$
\subitem b. Compute\ the\ error\ rate\ of\ $G_m(x)$\ over\ the\ training\ data:
\newline
\begin{equation}
e_m=P(G_m(x_i)\neq y_i)=\sum_{i=1}^N {w_{mi}\mathbb{I}(G_m(x_i)\neq y_i)}
\end{equation}

\subitem c. Compute the coefficient of leaner $G_m(x)$:
\begin{equation}
\alpha_m = \frac{1}{2}\log{\frac{1-e_m}{e_m}}
\end{equation}
\subitem d. Update\ the\ weights'\ distribution\ of\ training\ data:
\begin{equation}
w_{m+1,i}=\frac{w_{mi}}{Z_m}\exp(-\alpha_m y_i G_m(x_i))
\end{equation}
the\ normalizer\ $Z_m$:
\begin{equation}
Z_m=\sum_{i=1}^N w_{mi}\exp(-\alpha_m y_i G_m(x_i))
\end{equation}


\item Ensemble\ $M$\ weak\ learners:
\begin{equation}
G(x)=sign(\sum_{m=1}^M \alpha_m G_m(x))
\end{equation}
\end{enumerate} 

\section{The upper bound of the training error of AdaBoost}
\begin{theorem}
The upper bound of the training error of AdaBoost is :
\begin{equation}
\frac{1}{N} \sum_{i=1}^N \mathbb{I}(G(x_i)\neq y_i) \leq \frac{1}{N} \sum_{i=1}^N \exp(-y_i f(x_i))=\prod_{m=1}^M Z_m
\end{equation}

Note: the fooling equation would help proof this theorem:
\begin{equation}
w_{mi}\exp(-\alpha_m y_i G_m(x_i))=Z_m w_{m+1,i}
\end{equation}
\end{theorem}
